proving normal-order reduction may normalize is hard

vanilla.v
@@ -4,160 +4,6 @@ Require Import Coq.ZArith.BinInt.
 
 (** * De Bruijn Syntax of Terms *)
 
-Module IntShift.
-  Import Z.
-
-  Inductive expr : Set :=
-  | Var (z : Z)
-  | Lam (e : expr)
-  | App (e1 e2 : expr).
-  (**[]*)
-
-  Declare Scope expr_scope.
-  Delimit Scope expr_scope with expr.
-
-  Notation "'λ' e" := (Lam e) (at level 10) : expr_scope.
-  Notation "e1 ⋅ e2" := (App e1 e2) (at level 8, left associativity) : expr_scope.
-  Notation "! n" := (Var n) (at level 0) : expr_scope.
-
-  Open Scope expr_scope.
-  
-  Fixpoint shift (c i : Z) (e : expr) : expr :=
-    match e with
-    | !n =>  ! if (n <? c)%Z then n else n + i
-    | λ e => λ (shift (c + 1) i e)
-    | e1 ⋅ e2 => (shift c i e1) ⋅ (shift c i e2)
-    end.
-  (**[]*)
-
-  Lemma shift_up_down : forall e c i,
-      (0 < i)%Z ->
-      shift c (-i)%Z (shift c i e) = e.
-  Proof.
-    induction e as [z | e IHe | e1 IHe1 e2 IHe2];
-      intros; simpl; f_equal; auto.
-    destruct (z <? c)%Z eqn:Hzc; try rewrite Hzc; auto.
-    assert (Hzi: (z + i <? c)%Z = false).
-    { rewrite ltb_ge in *; lia. }
-    rewrite Hzi; lia.
-  Qed.
-
-  Lemma shift_down_up : forall e c i,
-      (0 < i)%Z ->
-      shift c i (shift c (-i)%Z e) = e.
-  Proof.
-    induction e as [z | e IHe | e1 IHe1 e2 IHe2];
-      intros; simpl; f_equal; auto.
-    destruct (z <? c)%Z eqn:Hzc; try rewrite Hzc; auto.
-  Abort.
-
-  Fixpoint sub (m : Z) (esub e : expr) : expr :=
-    match e with
-    | !n => if (m =? n)%Z then esub else !n
-    | λ e => λ (sub (m + 1) (shift 0 1 esub) e)
-    | e1 ⋅ e2 => (sub m esub e1) ⋅ (sub m esub e2)
-    end.
-  (**[]*)
-
-  Definition beta_reduce (e1 e2 : expr) : expr :=
-    shift 0 (-1)%Z (sub 0 (shift 0 1 e2) e1).
-  (**[]*)
-
-  Reserved Notation "e1 '-->' e2" (at level 40).
-
-  Inductive step : expr -> expr -> Prop :=
-  | step_beta e1 e2 :
-      (λ e1) ⋅ e2 -->  beta_reduce e1 e2
-  | step_lambda e e' :
-      e -->  e' ->
-      λ e -->  λ e'
-  | step_app_l e1 e1' e2 :
-      e1 -->  e1' ->
-      e1 ⋅ e2 -->  e1' ⋅ e2
-  | step_app_r e1 e2 e2' :
-      e2 -->  e2' ->
-      e1 ⋅ e2 -->  e1 ⋅ e2'
-  where "e1 '-->' e2" := (step e1 e2).
-  (**[]*)
-
-  Lemma shift_comm : forall e c1 i1 c2 i2,
-      shift c1 i1 (shift c2 i2 e) = shift c2 i2 (shift c1 i1 e).
-  Proof.
-    induction e; intros; simpl; f_equal; auto.
-    destruct (z <? c2)%Z eqn:Hzc2;
-      destruct (z <? c1)%Z eqn:Hzc1;
-      try rewrite Hzc1; try rewrite Hzc2; auto.
-  Abort.
-
-  Lemma shift_sub_shift : forall e1 e2 c1 i1 c2 i2,
-    (0 <= c1)%Z -> (0 <= c2)%Z -> (0 < i1)%Z -> (0 < i2)%Z ->
-    shift c1 i1 (shift c2 (-i2) (sub c2 (shift c2 i2 e2) e1)) =
-    shift c2 (-i2) (sub c2 (shift c2 i2 (shift c1 i1 e2)) (shift (c1 + 1) i1 e1)).
-  Proof.
-    induction e1; intros; simpl.
-    - admit.
-    - f_equal.
-  Abort.
-
-  Lemma shift_comm : forall e c1 i1 c2 i2,
-      (0 <= c1)%Z -> (0 <= c2)%Z -> (0 < i1)%Z -> (0 < i2)%Z ->
-      shift (c1 + 1) i1 (shift c2 i2 e) = shift c2 i2 (shift c1 i1 e).
-  Proof.
-    induction e; intros; simpl.
-    - destruct (z <? c2)%Z eqn:Hzc2;
-        destruct (z <? c1)%Z eqn:Hzc1;
-        repeat rewrite Hzc2; repeat rewrite Hzc1; f_equal;
-          try rewrite ltb_lt in *;
-          try rewrite ltb_ge in *.
-      + destruct (z <? c1 + 1)%Z eqn:Hzc11;
-          try rewrite ltb_ge in *; lia.
-      + destruct (z <? c1 + 1)%Z eqn:Hzc11;
-          destruct (z + i1 <? c2)%Z eqn:Hzi1c2;
-          try rewrite ltb_lt in *;
-          try rewrite ltb_ge in *; try lia; admit.
-      + admit.
-      + admit.
-    - f_equal; rewrite IHe by lia; reflexivity.
-    - rewrite IHe1 by lia;
-        rewrite IHe2 by lia; reflexivity.
-  Abort.
-
-  Lemma shift_sub_shift : forall e1 e2 c1 i1 c2 i2,
-      (0 <= c1)%Z -> (0 <= c2)%Z -> (0 < i1)%Z -> (0 < i2)%Z ->
-    shift c1 i1 (shift c2 (-i2) (sub c2 (shift 0 1 e2) e1)) =
-    shift c2 (-i2) (sub c2 (shift 0 1 (shift c1 i1 e2)) (shift (c1 + 1) i1 e1)).
-  Proof.
-    induction e1; intros; simpl.
-    - admit.
-    - f_equal. rewrite IHe1; simpl; f_equal; try lia.
-      do 2 f_equal.
-  Abort.
-  
-  Lemma shift_sub_shift : forall e1 e2 c i,
-    shift c i (shift 0 (-1) (sub 0 (shift 0 1 e2) e1)) =
-    shift 0 (-1) (sub 0 (shift 0 1 (shift c i e2)) (shift (c + 1) i e1)).
-  Proof.
-    induction e1; intros; simpl.
-    - admit.
-    - Fail rewrite <- IHe1.
-  Abort.
-    
-
-  Lemma step_shift : forall e e' c i,
-      e -->  e' ->
-      shift c i e -->  shift c i e'.
-  Proof.
-    Local Hint Constructors step : core.
-    intros e e' c i He;
-      generalize dependent i;
-      generalize dependent c;
-      induction He; intros; simpl; auto.
-    assert (H: shift c i (beta_reduce e1 e2) =
-               beta_reduce (shift (c + 1) i e1) (shift c i e2)).
-    { unfold beta_reduce.
-  Abort.
-End IntShift.
-
 Inductive expr : Set :=
 | Var (n : nat)
 | Lam (e : expr)
@@ -182,56 +28,9 @@ Fixpoint shift (op : nat -> nat) (c : nat) (e : expr) : expr :=
   end.
 (**[]*)
 
-Lemma shif_id : forall e c,
-    shift (fun n => n) c e = e.
-Proof.
-  induction e; intros; simpl; f_equal; auto.
-  destruct (n <? c); reflexivity.
-Qed.
-
-Lemma shift_compose : forall f h e c,
-    shift (compose f h) c e = compose (shift f c) (shift h c) e.
-Proof.
-  unfold compose. induction e; intros; simpl; f_equal; auto.
-  destruct (n <? c) eqn:Hnc; try rewrite Hnc; auto.
-Abort.
-
 Definition shift_up : expr -> expr := shift S 0.
 
 Definition shift_down : expr -> expr := shift pred 0.
-
-Lemma shift_c_down_comm : forall e c1 c2,
-    shift pred c1 (shift pred c2 e) = shift pred c2 (shift pred c1 e).
-Proof.
-  induction e; intros; simpl;  f_equal; auto.
-  (*destruct (n <? c2) eqn:Hc2; destruct (n <? c1) eqn:Hc1;
-    simpl; repeat rewrite Hc1; repeat rewrite Hc2; auto; unfold "$".
-    + assert (H: pred n <? c2 = true).
-      { rewrite Nat.ltb_lt in *. lia. }
-      rewrite H; reflexivity.
-    + assert (H: pred n <? c1 = true).
-      { rewrite Nat.ltb_lt in *. lia. }
-      rewrite H; reflexivity.
-    + destruct n as [| n]; simpl.
-      * destruct (0 <? c1); destruct (0 <? c2); reflexivity.
-      * rewrite Nat.ltb_ge in *.
-        Search (_ <? _ = negb (_ <=? _)).
-        repeat rewrite Nat.ltb_antisym.
-        Search (if (negb _) then _ else _).
-        repeat rewrite Bool.if_negb.
-        destruct (c1 <=? n) eqn:Hc1';
-          destruct (c2 <=? n) eqn:Hc2'; try reflexivity;
-            rewrite Nat.leb_le in *;
-            rewrite Nat.leb_gt in *.
-        ** assert (c2 = S n) by lia; subst. admit.
-        ** admit.*)
-Abort.
-
-Lemma shift_c_down_comm_0 : forall e c,
-    shift pred c (shift pred 0 e) = shift pred 0 (shift pred c e).
-Proof.
-  induction e; intros; simpl; f_equal; auto.
-Abort.
 
 Lemma shift_c_down_up : forall e c,
     shift pred c (shift S c e) = e.
@@ -260,28 +59,10 @@ Fixpoint sub (m : nat) (esub e : expr) : expr :=
   end.
 (**[]*)
 
-(*Lemma sub_shift_c_down_up : forall c m esub e,
-    shift pred c (sub m (shift S c m esub) e) =*)
-
 (** Beta-reduction [(λx.e1) e2 -> e1{e2/x}]. *)
 Definition beta_reduce (e1 e2 : expr) : expr :=
   shift_down (sub 0 (shift_up e2) e1).
 (**[]*)
-
-Lemma sub_beta_reduce : forall e1 e2 m es,
-    sub m es (beta_reduce e1 e2) =
-    beta_reduce
-      (sub (S m) (shift_up es) e1)
-      (sub m es e2).
-Proof.
-  unfold beta_reduce; simpl.
-  induction e1
-    as [ [| n1]
-       | e1 IHe1
-       | e11 IHe11 e21 IHe21 ]; intros; simpl.
-  - repeat rewrite shift_down_up. reflexivity.
-  - destruct (m =? n1) eqn:Hmn1; auto.
-Abort.
 
 Lemma shift_sub : forall e es m,
     shift pred m (sub m es (shift S m e)) = e.
@@ -301,218 +82,131 @@ Proof.
         rewrite H; reflexivity.
 Qed.
 
-Lemma sub_beta_c : forall e1 e2 es c m,
-  sub m es (shift pred c (sub c (shift S c e2) e1)) =
-  shift pred c (sub c (shift S c (sub m es e2)) (sub (S m) (shift S c es) e1)).
-Proof.
-  induction e1; intros e2 es c m; simpl; unfold shift_up.
-  - admit.
-  - f_equal. Fail rewrite <- IHe1. admit.
-  - f_equal; auto.
-Abort.
-  (*induction e1; intros [] es c m; simpl; unfold "$".
-  - destruct (c =? n) eqn:Hcn; destruct (n0 <? c) eqn:Hcn0;
-      destruct (m =? n0) eqn:Hmn0; destruct n as [| n];
-        simpl; repeat rewrite Hcn; repeat rewrite Hcn0;
-          repeat rewrite Hmn0; simpl; unfold "$"; admit.*)
-    (*+ rewrite shift_c_down_up; reflexivity.
-    + rewrite Nat.eqb_eq in *; subst.
-      destruct (n0 =? n) eqn:Hnn0; simpl.
-      * rewrite shift_sub. reflexivity.
-      * rewrite Nat.eqb_refl;
-          rewrite shift_c_down_up; reflexivity.
-    + rewrite Nat.eqb_eq in *; subst.
-      rewrite Nat.ltb_lt in Hcn0. lia.
-    + rewrite Nat.eqb_eq in *; subst.
-      destruct (m =? n) eqn:Hmn; simpl; auto.
-      * rewrite Nat.ltb_lt in *;
-          rewrite Nat.eqb_eq in *;
-          rewrite Nat.eqb_neq in *; subst. admit.
-      * rewrite Nat.eqb_refl; simpl; rewrite Hcn0; reflexivity.
-    +*) 
-  (*- destruct (c =? n) eqn:Hcn; destruct n as [| n];
-      simpl; unfold shift_up, "$"; try rewrite Hcn; simpl; unfold "$"; f_equal.
-    + repeat rewrite shift_c_down_up. reflexivity.
-    + rewrite Nat.eqb_eq in *; subst.
-      repeat rewrite shift_c_down_up.
-      destruct (m =? n) eqn:Hmn; simpl.
-      * rewrite Nat.eqb_eq in *; subst.
-        rewrite shift_sub. admit.
-      * rewrite Nat.eqb_refl; simpl; unfold "$"; f_equal.
-        rewrite shift_c_down_up. reflexivity.
-    + destruct (0 <? c) eqn:Hcn'; destruct (m =? 0) eqn:Hm0; auto; admit.
-    + destruct (S n <? c) eqn:HSnc;
-        destruct (m =? n) eqn:Hmn.
-      * rewrite Nat.eqb_eq in *; subst.
-        assert (HnSn: n =? S n = false).
-        { rewrite Nat.eqb_neq; lia. }
-        rewrite HnSn. rewrite shift_sub. admit.
-      * destruct (m =? S n) eqn:HmSn.
-        ** rewrite Nat.eqb_eq in *; subst.
-           simpl; rewrite Hcn; simpl; rewrite HSnc. admit.
-        ** simpl; rewrite Hcn; simpl; rewrite HSnc; reflexivity.
-      * rewrite Nat.eqb_eq in *; subst.
-        rewrite shift_sub. reflexivity.
-      * simpl; rewrite Hcn; simpl; rewrite HSnc; reflexivity.
-  - admit.
-  - admit.*)
-
 (** * Reduction Strategies *)
 
 (** Non-determistic reduction. *)
-Module NonDet.
-  Reserved Notation "e1 '-->' e2" (at level 40).
+Reserved Notation "e1 '-->' e2" (at level 40).
 
-  Inductive step : expr -> expr -> Prop :=
-  | step_beta e1 e2 :
-      (λ e1) ⋅ e2 -->  beta_reduce e1 e2
-  | step_lambda e e' :
-      e -->  e' ->
-      λ e -->  λ e'
-  | step_app_l e1 e1' e2 :
-      e1 -->  e1' ->
-      e1 ⋅ e2 -->  e1' ⋅ e2
-  | step_app_r e1 e2 e2' :
-      e2 -->  e2' ->
-      e1 ⋅ e2 -->  e1 ⋅ e2'
-  where "e1 '-->' e2" := (step e1 e2).
-  (**[]*)
+Inductive step : expr -> expr -> Prop :=
+| step_beta e1 e2 :
+    (λ e1) ⋅ e2 -->  beta_reduce e1 e2
+| step_lambda e e' :
+    e -->  e' ->
+    λ e -->  λ e'
+| step_app_l e1 e1' e2 :
+    e1 -->  e1' ->
+    e1 ⋅ e2 -->  e1' ⋅ e2
+| step_app_r e1 e2 e2' :
+    e2 -->  e2' ->
+    e1 ⋅ e2 -->  e1 ⋅ e2'
+where "e1 '-->' e2" := (step e1 e2).
+(**[]*)
 
-  Notation "e1 '-->*' e2" := (refl_trans_closure step e1 e2) (at level 40).
+(** No beta-reduxes. *)
+Inductive normal_form : expr -> Prop :=
+| nf_var n :
+    normal_form !n
+| nf_app n e :
+    normal_form e ->
+    normal_form (!n ⋅ e)
+| nf_lam e :
+    normal_form e ->
+    normal_form (λ e).
+(**[]*)
 
-  Section Conf.
-    Local Hint Constructors step : core.
+Section NormalForm.
+  Theorem normal_form_step : forall e e',
+    normal_form e -> ~ e -->  e'.
+  Proof.
+    intros e e' HN; generalize dependent e';
+      induction HN; intros ? H'; inv H'.
+    - inv H2.
+    - apply IHHN in H2; contradiction.
+    - apply IHHN in H0; contradiction.
+  Qed.
+End NormalForm.
 
-    Lemma shift_up_down_c_comm : forall e c1 c2,
-        c2 <= c1 ->
-        shift S c1 (shift pred c2 e) = shift pred c2 (shift S c1 e).
-    Proof.
-      induction e as [n | e IHe | e1 IHe1 e2 IHe2]; intros; simpl; f_equal; auto.
-      destruct (n <? c2) eqn:Hnc2; destruct (n <? c1) eqn:Hnc1;
-        try rewrite Hnc2; try rewrite Hnc1; auto.
-      - destruct (S n <? c2) eqn:HSnc2; simpl; auto.
-        rewrite Nat.ltb_lt in *; rewrite Nat.ltb_ge in *; lia.
-      - destruct (pred n <? c1) eqn:Hpnc1; simpl; auto.
-        rewrite Nat.ltb_lt in *; rewrite Nat.ltb_ge in *; lia.
-      - destruct (S n <? c2) eqn:HSnc2;
-          destruct (pred n <? c1) eqn:Hpnc1; simpl; auto;
-            try rewrite Nat.ltb_lt in *; try rewrite Nat.ltb_ge in *; try lia.
-        + destruct n; simpl in *; try lia. admit.
-        + destruct n; simpl in *; try lia. admit.
-      - rewrite IHe by lia. reflexivity.
-    Abort.
-        
+Notation "e1 '-->*' e2" := (refl_trans_closure step e1 e2) (at level 40).
 
-    Lemma shift_up_c_reduce : forall e e' c,
-        e -->  e' -> shift S c e -->  shift S c e'.
-    Proof.
-      intros e e' c H; generalize dependent c;
-        induction H; intros; simpl; auto.
-      assert (shift S c (beta_reduce e1 e2) =
-              beta_reduce (shift S (S c) e1) (shift S c e2)).
-      { unfold beta_reduce, shift_down, shift_up.
-    Abort.    
-      
-    Lemma sub_reduce_sub : forall e e' es m,
-        e -->  e' -> sub m es e -->  sub m es e'.
-    Proof.
-      intros e e' es m H; generalize dependent m;
-        generalize dependent es;
-        induction H; intros es m;
-          simpl; eauto.
-      assert (sub m es (beta_reduce e1 e2) =
-              beta_reduce (sub (S m) (shift_up es) e1) (sub m es e2)).
-      { unfold beta_reduce, shift_down, shift_up.
-        induction e1; simpl.
-        - admit.
-        - f_equal. Fail rewrite <- IHe1. admit.
-        - f_equal; auto.
-    Abort.
+(** Termination condition. *)
+Definition halts (e e' : expr) : Prop :=
+  e -->* e' /\ normal_form e'.
 
-    Lemma shift_pred_reduce : forall e e' c,
-        e -->  e' -> shift pred c e -->  shift pred c e'.
-    Proof.
-      intros e e' c H; generalize dependent c;
-        induction H; intros c; simpl; auto.
-      unfold beta_reduce, shift_down.
-    Abort.
+Section Confluence.
+  Local Hint Constructors step : core.    
+  Local Hint Resolve inject_trans_closure : core.
+  Local Hint Resolve refl_closure : core.
 
-    Lemma shift_sub_reduce_term : forall e1 e2 e c,
-        e1 -->  e2 ->
-        shift pred c (sub c e e1) -->  shift pred c (sub c e e2).
-    Proof.
-      intros e1 e2 e c H; generalize dependent c;
-        generalize dependent e;
-        induction H; intros; simpl; auto.
-      - assert (shift pred c (sub c e (beta_reduce e1 e2)) =
-                beta_reduce
-                  (shift pred (S c) (sub (S c) (shift_up e) e1))
-                  (shift pred c (sub c e e2))).
-        { unfold beta_reduce, shift_up, shift_down; simpl.
-    Abort.
-    
-    Lemma beta_reduce_subterm_l : forall e1 e2 e,
-        e1 -->  e2 ->
-        beta_reduce e1 e -->  beta_reduce e2 e.
-    Proof.
-      intros e1 e2 e H; generalize dependent e;
-        induction H; intros;
-          unfold beta_reduce, shift_down, shift_up; simpl in *; auto.
-      - admit.
-      - constructor. admit.
-    Abort.
-    
-    Local Hint Resolve inject_trans_closure : core.
-    Local Hint Resolve refl_closure : core.
+  Lemma reduce_lambda : forall e e',
+      e -->* e' -> λ e -->* λ e'.
+  Proof.
+    intros e e' H; induction H; auto 1.
+    transitivity (λ a2); auto 3.
+  Qed.
 
-    Lemma reduce_lambda : forall e e',
-        e -->* e' -> λ e -->* λ e'.
-    Proof.
-      intros e e' H; induction H; auto 1.
-      transitivity (λ a2); auto 3.
-    Qed.
+  Lemma reduce_app_l : forall e1 e1' e2,
+      e1 -->* e1' -> e1 ⋅ e2 -->* e1' ⋅ e2.
+  Proof.
+    intros e1 e1' e2 H; induction H; auto 1.
+    transitivity (a2 ⋅ e2); auto 3.
+  Qed.
 
-    Lemma reduce_app_l : forall e1 e1' e2,
-        e1 -->* e1' -> e1 ⋅ e2 -->* e1' ⋅ e2.
-    Proof.
-      intros e1 e1' e2 H; induction H; auto 1.
-      transitivity (a2 ⋅ e2); auto 3.
-    Qed.
+  Lemma reduce_app_r : forall e1 e2 e2',
+      e2 -->* e2' -> e1 ⋅ e2 -->* e1 ⋅ e2'.
+  Proof.
+    intros e1 e2 e2' H; induction H; auto 1.
+    transitivity (e1 ⋅ a2); auto 3.
+  Qed.
 
-    Lemma reduce_app_r : forall e1 e2 e2',
-        e2 -->* e2' -> e1 ⋅ e2 -->* e1 ⋅ e2'.
-    Proof.
-      intros e1 e2 e2' H; induction H; auto 1.
-      transitivity (e1 ⋅ a2); auto 3.
-    Qed.
+  Local Hint Resolve reduce_lambda : core.
+  Local Hint Resolve reduce_app_l : core.
+  Local Hint Resolve reduce_app_r : core.
 
-    Local Hint Resolve reduce_lambda : core.
-    Local Hint Resolve reduce_app_l : core.
-    Local Hint Resolve reduce_app_r : core.
+  Conjecture beta_reduce_inner_l : forall e1 e1' e2,
+      e1 -->  e1' -> beta_reduce e1 e2 -->* beta_reduce e1' e2.
 
-    Theorem confluence : forall e e1 e2,
-        e -->  e1 -> e -->  e2 -> exists e', e1 -->* e' /\ e2 -->* e'.
-    Proof.
-      intros ? ? e2 H1;
-        generalize dependent e2;
-        induction H1; intros ? H2; inv H2; eauto 3.
-      - inv H3. exists (beta_reduce e' e2); split; auto. admit.
-      - exists (beta_reduce e1 e2'); split; auto. admit.
-      - pose proof IHstep _ H0 as [? [? ?]]; eauto.
-      - inversion H1; subst.
-        pose proof IHstep _ H1 as [? [? ?]]; clear IHstep.
-        exists (beta_reduce e' e2); split; auto. admit.
-      - pose proof IHstep _ H4 as [? [? ?]]; eauto.
-      - clear IHstep. exists (e1' ⋅ e2'); split; eauto.
-      - clear IHstep. exists (beta_reduce e3 e2'); split; auto. admit.
-      - clear IHstep. exists (e1' ⋅ e2'); split; eauto.
-      - pose proof IHstep _ H4 as [? [? ?]]; eauto.
-    Admitted.
-End Conf.        
-End NonDet.
+  Conjecture beta_reduce_inner_r : forall e1 e2 e2',
+      e2 -->  e2' -> beta_reduce e1 e2 -->* beta_reduce e1 e2'.
+  
+  Theorem confluence : forall e e1 e2,
+      e -->  e1 -> e -->  e2 -> exists e', e1 -->* e' /\ e2 -->* e'.
+  Proof.
+    intros ? ? e2 H1;
+      generalize dependent e2;
+      induction H1; intros ? H2; inv H2; eauto 3.
+    - inv H3; exists (beta_reduce e' e2); split; auto.
+      apply beta_reduce_inner_l; assumption.
+    - exists (beta_reduce e1 e2'); split; auto.
+      apply beta_reduce_inner_r; assumption.
+    - pose proof IHstep _ H0 as [? [? ?]]; eauto.
+    - inversion H1; subst.
+      pose proof IHstep _ H1 as [? [? ?]]; clear IHstep.
+      exists (beta_reduce e' e2); split; auto.
+      apply beta_reduce_inner_l; assumption.
+    - pose proof IHstep _ H4 as [? [? ?]]; eauto.
+    - clear IHstep. exists (e1' ⋅ e2'); split; eauto.
+    - clear IHstep. exists (beta_reduce e3 e2'); split; auto.
+      apply beta_reduce_inner_r; assumption.
+    - clear IHstep. exists (e1' ⋅ e2'); split; eauto.
+    - pose proof IHstep _ H4 as [? [? ?]]; eauto.
+  Qed.
+
+  Local Hint Resolve confluence : core.
+  Local Hint Constructors refl_trans_closure : core.
+
+  Corollary confluence_star :  forall e e1 e2,
+      e -->* e1 -> e -->* e2 -> exists e', e1 -->* e' /\ e2 -->* e'.
+  Proof.
+    (*intros ? ? ? He1 He2; inv He1; inv He2; eauto.*)
+    (*intros e e1 e2 He1; generalize dependent e2;
+      induction He1; intros ? He2; inv He2; eauto.
+    apply IHHe1.
+    pose proof IHHe1 _ He1 as [e' [He1' He2']].*)
+  Abort.
+End Confluence.
 
 (** Deterministic reduction. *)
-Module Det.
+
 Inductive shallow_value : expr -> Prop :=
 | shl_var n : shallow_value !n
 | shl_lam e : shallow_value (λ e).
@@ -537,20 +231,20 @@ Inductive deep_value : expr -> Prop :=
 
 (** Call-by-value. *)
 
-Reserved Notation "e1 '-->' e2" (at level 40).
+Reserved Notation "e1 '⟶' e2" (at level 40).
 
 Inductive cbv_reduce : expr -> expr -> Prop :=
 | cbv_beta e1 e2 :
     shallow_value e2 ->
-    (λ e1) ⋅ e2 -->  beta_reduce e1 e2
-| cbv_right e1 e2 e2' :
+    (λ e1) ⋅ e2 ⟶  beta_reduce e1 e2
+| cbv_app_r e1 e2 e2' :
     shallow_value e1 ->
-    e2 -->  e2' ->
-    e1 ⋅ e2 -->  e1 ⋅ e2'
-| cbv_left e1 e1' e2 :
-    e1 -->  e1' ->
-    e1 ⋅ e2 -->  e1' ⋅ e2
-where "e1 '-->' e2" := (cbv_reduce e1 e2).
+    e2 ⟶  e2' ->
+    e1 ⋅ e2 ⟶  e1 ⋅ e2'
+| cbv_app_l e1 e1' e2 :
+    e1 ⟶  e1' ->
+    e1 ⋅ e2 ⟶   e1' ⋅ e2
+where "e1 '⟶' e2" := (cbv_reduce e1 e2).
 
 (** Call-by-name. *)
 
@@ -559,7 +253,7 @@ Reserved Notation "e1 '==>' e2" (at level 40).
 Inductive cbn_reduce : expr -> expr -> Prop :=
 | cbn_beta e1 e2 :
     (λ e1) ⋅ e2 ==>  beta_reduce e1 e2
-| cbn_step e1 e1' e2 :
+| cbn_app_l e1 e1' e2 :
     e1 ==>  e1' ->
     e1 ⋅ e2 ==>  e1' ⋅ e2
 where "e1 '==>' e2" := (cbn_reduce e1 e2).
@@ -574,10 +268,10 @@ Inductive normal_reduce : expr -> expr -> Prop :=
 | normal_lambda e e' :
     e >-> e' ->
     λ e >-> λ e'
-| normal_right n e2 e2' :
+| normal_app_r n e2 e2' :
     e2 >-> e2' ->
     !n ⋅ e2 >-> !n ⋅ e2'
-| normal_left e1 e1' e2 :
+| normal_app_l e1 e1' e2 :
     ~ is_lambda e1 ->
     e1 >-> e1' ->
     e1 ⋅ e2 >-> e1' ⋅ e2
@@ -595,11 +289,11 @@ Inductive appl_reduce : expr -> expr -> Prop :=
 | appl_lambda e e' :
     e ⇢ e' ->
     λ e ⇢ λ e'
-| appl_right e1 e2 e2' :
+| appl_app_r e1 e2 e2' :
     deep_value e1 ->
     e2 ⇢ e2' ->
     e1 ⋅ e2 ⇢ e1 ⋅ e2'
-| appl_left e1 e1' e2 :
+| appl_app_l e1 e1' e2 :
     e1 ⇢ e1' ->
     e1 ⋅ e2 ⇢ e1' ⋅ e2
 where "e1 '⇢' e2" := (appl_reduce e1 e2).
@@ -614,7 +308,7 @@ Ltac not_is_lambda_lambda :=
 
 Ltac cbv_step_lambda :=
   match goal with
-  | H: λ _ -->  _ |- _ => inv H
+  | H: λ _ ⟶  _ |- _ => inv H
   end.
 (**[]*)
 
@@ -634,7 +328,7 @@ Section Shallow.
   Local Hint Constructors shallow_value : core.
 
   Lemma cbv_reduce_value : forall e e',
-      e -->  e' -> ~ shallow_value e.
+      e ⟶   e' -> ~ shallow_value e.
   Proof. intros ? ? H Hv; inv H; inv Hv. Qed.
 
   Lemma cbn_reduce_value : forall e e',
@@ -661,7 +355,7 @@ End Deep.
 
 Ltac contra_cbv_value :=
   match goal with
-  | H: ?e -->  _, Hv: shallow_value ?e
+  | H: ?e ⟶  _, Hv: shallow_value ?e
     |- _ => apply cbv_reduce_value in H; contradiction
   end.
 (**[]*)
@@ -760,40 +454,70 @@ Section ValueEXM.
   Qed.
 End ValueEXM.
 
-Notation "e1 '-->*' e2" := (refl_trans_closure cbv_reduce e1 e2) (at level 40).
-Notation "e1 '==>*' e2" := (refl_trans_closure cbn_reduce e1 e2) (at level 40).
+Section InjectStep.
+  Local Hint Constructors step : core.
 
-Section Confluence.
-  Local Hint Resolve refl_closure : core.
+  Theorem cbv_step : forall e e', e ⟶  e' -> e -->  e'.
+  Proof. intros ? ? H; induction H; auto 2. Qed.
+
+  Theorem cbn_step : forall e e', e ==>  e' -> e -->  e'.
+  Proof. intros ? ? H; induction H; auto 2. Qed.
+
+  Theorem normal_step : forall e e', e >-> e' -> e -->  e'.
+  Proof. intros ? ? H; induction H; auto 2. Qed.
+
+  Theorem appl_step : forall e e', e ⇢ e' -> e -->  e'.
+  Proof. intros ? ? H; induction H; auto 2. Qed.
+End InjectStep.
+
+Notation "e1 >->* e2" := (refl_trans_closure normal_reduce e1 e2) (at level 40).
+
+Section Normalizing.
   Local Hint Resolve inject_trans_closure : core.
+  Local Hint Resolve refl_closure : core.
+  Local Hint Constructors normal_reduce : core.
+
+  Lemma normal_reduce_lambda : forall e e',
+      e >->* e' -> λ e >->* λ e'.
+  Proof.
+    intros e e' H; induction H; auto 1.
+    transitivity (λ a2); auto 3.
+  Qed.
+
+  Lemma normal_reduce_app_l : forall e1 e1' e2,
+      e1 >->* e1' -> e1 ⋅ e2 >->* e1' ⋅ e2.
+  Proof.
+    intros e1 e1' e2 H; induction H; auto 1.
+    transitivity (a2 ⋅ e2); auto 3.
+    apply inject_trans_closure.
+    apply normal_app_l.
+  Abort.
+
+  Lemma normal_reduce_app_r : forall e1 e2 e2',
+      e2 >->* e2' -> e1 ⋅ e2 >->* e1 ⋅ e2'.
+  Proof.
+    intros e1 e2 e2' H; induction H; auto 1.
+    transitivity (e1 ⋅ a2); auto 3.
+  Abort.
+
+  Local Hint Resolve normal_reduce_lambda : core.
+  (*Local Hint Resolve normal_reduce_app_l : core.*)
+  (*Local Hint Resolve normal_reduce_app_r : core.*)
+  Local Hint Constructors normal_form : core.
   
-  Section CBV_CBN.
-    Local Hint Extern 0 => cbv_step_lambda : core.
-    Local Hint Extern 0 => cbn_step_lambda : core.
-    Local Hint Constructors cbv_reduce : core.
-    Local Hint Constructors cbn_reduce : core.
-    Local Hint Extern 0 => contra_cbn_value : core.
-    
-    Theorem cbv_cbn_confluent : forall e e1 e2,
-      e -->  e1 -> e ==>  e2 -> exists e', e1 -->* e' /\ e2 ==>* e'.
-    Proof.
-      intros e e1 e2 Hcbv.
-      generalize dependent e2.
-      induction Hcbv; intros ? Hcbn; inv Hcbn; eauto 3.
-      - clear IHHcbv; destruct (shallow_value_exm e2') as [Hv | Hv].
-        + exists (beta_reduce e3 e2'). split.
-          * apply trans_closure with (beta_reduce e3 e2'); auto 2.
-          * unfold beta_reduce, "$". admit.
-        + admit.
-      - apply IHHcbv in H2 as [e'' [Hcbv' Hcbn']]; clear IHHcbv.
-        exists (e'' ⋅ e2); split.
-        + clear e1 e1'0 Hcbn' Hcbv.
-          induction Hcbv'; auto 1.
-          transitivity (a2 ⋅ e2); auto 3.
-        + clear e1 e1' Hcbv Hcbv'.
-          induction Hcbn'; auto 1.
-          transitivity (a2 ⋅ e2); auto 3.
-    Admitted.
-  End CBV_CBN.
-End Confluence.
-End Det.
+  Theorem normal_halts : forall e e',
+    halts e e' -> e >->* e'.
+  Proof.
+    intros e e' [He Hnf].
+    induction He; inv Hnf; auto.
+    - assert (a2 >->* !n) by auto; clear IHHe.
+      (*assert (exists a2', a1 >->* a2' /\ a2' >->* a2).
+      + transitivity (beta_reduce e1 e2); auto.
+      + transitivity (λ e'); auto.
+        apply inject_trans_closure; constructor. admit.
+      + transitivity (e1' ⋅ e2); auto.
+        apply inject_trans_closure. *) admit.
+    - assert (a2 >->* !n ⋅ e) by auto; clear IHHe. admit.
+    - assert (a2 >->* λ e) by auto; clear IHHe. admit.
+  Abort.
+End Normalizing.
